updating tests

tests/micro-benchmarks/Unit1.WPsAndTriples.fst
@@ -39,11 +39,27 @@ let g = h (as_Pure f)
  *)
 
 [@@ expect_failure]
-val bad_wp : unit -> PURE unit (fun p -> ~ (p ()))
+val bad_wp : unit -> PURE unit (as_pure_wp (fun p -> ~ (p ())))
 
-[@@expect_failure]
-val bad_wp : unit -> PURE int (fun p -> ~ (p 3))
+[@@ expect_failure]
+val bad_wp : unit -> PURE int (as_pure_wp (fun p -> ~ (p 3)))
 
 
 val good_wp : unit -> PURE int (as_pure_wp (fun p -> p 3))
 val good_hoare : unit -> Pure int True (fun r -> r == 3)
+
+(*
+ * An example from Dominique Unruh
+ *)
+let mono a (wp:pure_wp a) (p q:pure_post a) (_:squash(forall (x:a). p x ==> q x)) : 
+    Lemma (wp p ==> wp q) = 
+	FStar.Monotonic.Pure.elim_pure_wp_monotonicity_forall ()
+
+[@@ expect_failure]
+let contradiction () : Lemma(False) = 
+    let a = unit in
+    let wp : pure_wp a = as_pure_wp (fun p -> ~ (p ())) in
+    let p x = False in let q x = True in
+    let u : squash(forall x. p x ==> q x) = () in
+    mono a wp p q u;
+    assert (wp p ==> wp q)
